tests/test10st_metatheoryScript.sml
@@ -62,7 +62,7 @@ Induct THEN RW_TAC list_ss [GtT_fun, is_v_of_t_def]);
 val progress_thm = Q.prove (
 `!G t Ty. GtT G t Ty ==> (G = []) ==> is_v_of_t t \/ ?t'. reduce t t'`,
 RI GtT_sind THEN IMP_RES_TAC canon_val_lem THEN RW_TAC list_ss [reduce_fun, GtT_fun, is_v_of_t_def] THEN
-METIS_TAC [lookup_def, NOT_SOME_NONE, is_v_of_t_def]);
+METIS_TAC [lookup_def, NOT_SOME_NONE, is_v_of_t_def, clause_name_def]);
 
 val context_lem = Q.prove (
 `!G t Ty. GtT G t Ty ==> 
